higherlower2/C/C.fst
@@ -6,17 +6,41 @@ $ make main.ocaml.exe
 
 module C
 
-open CallbackImpl
 open GeneratedProto1C
 open Payload
 open Network
 
 open FStar.Tcp
+open FStar.Error
 
 let ip_addr_B = "127.0.0.1"
 let port_B = 5000
 
-let mk_comms stream : communications = {
+(*
+type label =
+| Guess
+| Higher
+| Lose
+| Lower
+| Win
+*)
+
+let encode_label = function
+  | Guess -> 0
+  | Higher -> 1
+  | Lose -> 2
+  | Lower -> 3
+  | Win -> 4
+
+let decode_label = function
+  | 0 -> Guess
+  | 1 -> Higher
+  | 2 -> Lose
+  | 3 -> Lower
+  | 4 -> Win
+  | _ -> unexpected "Unexpected Label"
+
+let mk_comms stream : connection = {
   send_int = (fun _role p ->
     let p = payload_of_int p in
     send_payload stream p);
@@ -26,6 +50,9 @@ let mk_comms stream : communications = {
   send_unit = (fun _role p ->
     let p = payload_of_unit p in
     send_payload stream p);
+  send_label = (fun _role l ->
+    let l = encode_label l in
+    send_payload stream (Int l));
   recv_int = (fun _role _ ->
     let p = recv_payload stream in
     int_of_payload p);
@@ -35,10 +62,19 @@ let mk_comms stream : communications = {
   recv_unit = (fun _role _ ->
     let p = recv_payload stream in
     unit_of_payload p);
+  recv_label = (fun _role _ ->
+    let p = recv_payload stream in
+    decode_label (int_of_payload p));
 }
 
 let main () =
     let server_B = connect ip_addr_B port_B in
     let comms = mk_comms server_B in
-    let () = run callbacks comms in
+    let () = run CallbackImpl.callbacks comms in
+    close server_B
+
+let main_alt () =
+    let server_B = connect ip_addr_B port_B in
+    let comms = mk_comms server_B in
+    let () = run CallbackImplAlt.callbacks comms in
     close server_B
